Remove some useless lemmas, and update some lemmas.

src/PFuncAbstractDomain.v
@@ -26,7 +26,7 @@ Module PFuncMap (FPI: FPresburgerImpl).
   Qed.
 
   Theorem to_var_values_seq_update_neq :
-    forall p R v c i, i != index v (vars_in_program p) ->
+    forall p R v c i, i <> index v (vars_in_program p) ->
       nth 0%Z (to_var_values_seq p (v !-> c; R)) i =
       nth 0%Z (to_var_values_seq p R) i.
   Proof.
@@ -37,7 +37,7 @@ Module PFuncMap (FPI: FPresburgerImpl).
     rewrite !(nth_map ""); try (by []).
     apply t_update_neq.
     apply /eqP => Hv. subst. rewrite index_uniq in Hindex; autossr.
-      by move => /eqP in Hindex.
+      by [].
       by apply uniq_vars_in_program.
   Qed.
 
@@ -82,7 +82,7 @@ Module PFuncMap (FPI: FPresburgerImpl).
     let vars := vars_in_program p in
     to_var_values_map_ p (zip vars s).
 
-  Theorem to_var_values_mapP :
+  Theorem to_var_values_map_index :
     forall p s i, i < size (vars_in_program p) ->
              (to_var_values_map p s) (nth "" (vars_in_program p) i) =
              nth 0%Z s i.
@@ -112,12 +112,22 @@ Module PFuncMap (FPI: FPresburgerImpl).
       rewrite leqNgt. by rewrite Hsize.
   Qed.
 
+  Theorem to_var_values_mapP :
+    forall p s v, v \in (vars_in_program p) ->
+                   (to_var_values_map p s) v =
+                   nth 0%Z s (index v (vars_in_program p)).
+  Proof.
+    move => p s v Hin.
+    rewrite <-(to_var_values_map_index p); last by rewrite index_mem.
+    by rewrite nth_index.
+  Qed.
+
   Theorem to_var_values_map_equality :
     forall p s, point_equality (size (vars_in_program p)) s (to_var_values_seq p (to_var_values_map p s)).
   Proof.
     move => p s. apply /allP => i Hiota. simplssr.
     rewrite /to_var_values_seq (nth_map "") => //.
-    by rewrite to_var_values_mapP.
+    by rewrite to_var_values_map_index.
   Qed.
 
   Theorem to_var_values_map_equality_sym :
@@ -156,26 +166,26 @@ Module PFuncMap (FPI: FPresburgerImpl).
     - subst. rewrite nth_index; auto_map.
     - rewrite t_update_neq; last first. apply /eqP => Hv. subst.
         rewrite index_uniq in Hi. by []. by simplssr. by apply uniq_vars_in_program.
-      rewrite to_var_values_mapP; by autossr.
+      rewrite to_var_values_map_index; by autossr.
   Qed.
 
   Definition PFuncMap (p: Program) :=
     let n := size (vars_in_program p) in
     { x: seq (PFunc_eqType n) | size x == n}.
 
-  Program Definition bot_PFuncMap (p: Program) : PFuncMap p :=
-    let n := size (vars_in_program p) in
-    (nseq n (constant_pfunc n VBot)).
+  Program Definition nseq_pfuncmap (p: Program) (pf: PFunc (size (vars_in_program p))) : PFuncMap p :=
+    nseq (size (vars_in_program p)) pf.
   Next Obligation.
-      by rewrite size_nseq.
-  Qed.
+    by rewrite size_nseq.
+  Defined.
 
-  Program Definition top_PFuncMap (p: Program) : PFuncMap p :=
+  Definition bot_PFuncMap (p: Program) : PFuncMap p :=
     let n := size (vars_in_program p) in
-    nseq n (constant_pfunc n VTop).
-  Next Obligation.
-      by rewrite size_nseq.
-  Qed.
+    nseq_pfuncmap p (constant_pfunc n VBot).
+
+  Definition top_PFuncMap (p: Program) : PFuncMap p :=
+    let n := size (vars_in_program p) in
+    nseq_pfuncmap p (constant_pfunc n VTop).
 
   Program Definition join_PFuncMap {p: Program} (p1 p2: PFuncMap p) : PFuncMap p :=
     [ seq join_pfunc x.1 x.2 | x <- zip p1 p2].
@@ -348,6 +358,22 @@ Module PFuncMap (FPI: FPresburgerImpl).
     - move => acc a. rewrite /A. by simpl_pfunc.
   Qed.
 
+  Theorem get_unioned_bot_set_indexP :
+    forall n (pf: seq (PFunc n)) x,
+      x \in (get_unioned_bot_set pf) =
+      has (fun i => x \in (pfunc_get_bot_set (nth (constant_pfunc _ VTop) pf i))) (iota 0 (size pf)).
+  Proof.
+    move => n pf x. rewrite get_unioned_bot_setP.
+    apply /idP/idP.
+    - move => /hasP [pfunc Hin Hin_bot]. apply /hasP.
+      exists (index pfunc pf). simplssr.
+      + by rewrite -index_mem in Hin.
+      + by rewrite nth_index.
+    - move => /hasP [i Hiota Hin_bot]. apply /hasP.
+      exists (nth (constant_pfunc _ VTop) pf i) => //.
+      apply mem_nth. by autossr.
+  Qed.
+
   Theorem get_unioned_bot_set_pfuncmapP :
     forall p pf x_in, (to_var_values_seq p x_in) \in (get_unioned_bot_set (sval pf)) <-> forall x_out, ~ (In _ (@gamma_PFuncMap p pf) (x_in, x_out)).
   Proof.
@@ -366,11 +392,38 @@ Module PFuncMap (FPI: FPresburgerImpl).
       move: HIn => /(_ x_out_map) /negP /allPn [i Hi Hnotin].
       move: Hi. rewrite mem_iota => /andP[_ Hi]. rewrite add0n in Hi.
       rewrite {1}/to_var_values_seq (nth_map "") in Hnotin => //.
-      rewrite /x_out_map to_var_values_mapP /x_out in Hnotin => //.
+      rewrite /x_out_map to_var_values_map_index /x_out in Hnotin => //.
       erewrite (nth_map top_pfunc) in Hnotin; last by rewrite H_pf.
       move: Hnotin. case Heval: (eval_pfunc _ _) => [ // | n | ]. by simpl_pfunc.
       move => _. exists (nth top_pfunc x_pf i). apply mem_nth. by rewrite H_pf.
         by rewrite pfunc_get_bot_setP Heval.
+  Qed.
+
+  Theorem get_unioned_bot_set_pfuncmap_intro :
+    forall p pf x_in x_out, (In _ (@gamma_PFuncMap p pf) (x_in, x_out)) ->
+                       (to_var_values_seq p x_in) \notin (get_unioned_bot_set (sval pf)).
+  Proof.
+    move => p pf x_in x_out HIn.
+    apply /negP => Hin.
+    apply get_unioned_bot_set_pfuncmapP in HIn => //.
+  Qed.
+
+  Theorem get_unioned_bot_set_pw_aff_some :
+    forall p (pf: PFuncMap p) x_in_map,
+      let default := constant_pfunc _ VTop in
+      let x_in := to_var_values_seq p x_in_map in
+      (x_in \notin (get_unioned_bot_set (sval pf))) ->
+      forall i, i < size (vars_in_program p) ->
+        x_in \in Assumed (nth default (sval pf) i) ->
+        exists x_out, f_eval_pw_aff (Val (nth default (sval pf) i)) (x_in) = Some x_out.
+  Proof.
+    move => p pf x_in_map default x_in Hx_notin i Hi Hassumed.
+    exists (match f_eval_pw_aff (Val (nth default (sval pf) i)) x_in with | Some v => v | _ => 0%Z end).
+    case_match => //.
+    move => /negP /get_unioned_bot_set_pfuncmapP in Hx_notin.
+    have Hiota: (i \in iota 0 (size (vars_in_program p))). autossr.
+    exfalso. apply Hx_notin => x_out /allP /(_ i Hiota) /=.
+    rewrite /eval_pfunc. by rewrite Hassumed H.
   Qed.
 
   Definition get_result_pfuncmap {p: Program} (pf: PFuncMap p) (x_in: seq Z) :=
@@ -718,221 +771,5 @@ Module PFuncMap (FPI: FPresburgerImpl).
       compose_transitive_closure_bot := (compose_transitive_closure_bot_PFuncMap p);
       compose_transitive_closure_le := (compose_transitive_closure_le_PFuncMap p);
     }.
-
-  Program Definition transfer_inst_const_PFuncMap {p: Program} (pf: PFuncMap p) (v: vid) (c: Z) : PFuncMap p :=
-    let id := index v (vars_in_program p) in
-    if id >= (size (vars_in_program p)) then
-      sval pf
-    else
-      let bot_set := get_unioned_bot_set (sval pf) in
-      let const_pfunc := constant_pfunc _ (VVal c) in
-      let const_pfunc_val := f_intersect_domain (Val const_pfunc) (f_complement_set bot_set) in
-      let const_pfunc' := mkPFunc const_pfunc_val (Assumed const_pfunc) in
-      set_nth (constant_pfunc _ VTop) pf id const_pfunc'.
-  Next Obligation.
-    case_if.
-    - by case: pf => x_pf /= /eqP ->.
-    - rewrite size_set_nth.
-      case: pf => x_pf /= /eqP ->. apply /eqP.
-      apply /maxn_idPr.
-      move => /negb_true_iff in H.
-        by rewrite ltnNge.
-  Qed.
-
-  Theorem transfer_inst_PFuncMap_not_in_program :
-    forall p v c (pf: PFuncMap p),
-      index v (vars_in_program p) >= (size (vars_in_program p)) ->
-      transfer_inst_const_PFuncMap pf v c = pf.
-  Proof.
-    move => p v c pf H.
-    rewrite /transfer_inst_const_PFuncMap.
-      by apply val_inj; rewrite /= H.
-  Qed.
-
-  Theorem transfer_inst_const_PFuncMap_exists :
-    forall p (pf: PFuncMap p) v c x_in x_out,
-      In _ (gamma (transfer_inst_const_PFuncMap pf v c)) (x_in, x_out) ->
-      exists c', In _ (gamma pf) (x_in, (v !-> c'; x_out)).
-  Proof.
-    move => p pf v c x_in x_out HIn.
-    case Hindex: (index v (vars_in_program p) >= (size (vars_in_program p))).
-    - exists (x_out v). rewrite transfer_inst_PFuncMap_not_in_program in HIn => //.
-      apply /allP => i Hiota /=. rewrite /to_var_values_seq.
-      setoid_rewrite t_update_same.
-      by move => /allP /(_ i Hiota) in HIn.
-    - rewrite /transfer_inst_const_PFuncMap /= in HIn.
-      set pfunc := (nth (constant_pfunc _ VTop) (sval pf) (index v (vars_in_program p))).
-      exists (match eval_pfunc pfunc (to_var_values_seq p x_in) with | VVal z => z | _ => 0%Z end).
-      apply /allP => i Hiota. move: HIn => /allP /(_ i Hiota) /=.
-      rewrite Hindex nth_set_nth /=.
-      case: (i =P index v (vars_in_program p)) => Hi.
-      + subst. move => HIn. rewrite /eval_pfunc in HIn. move: HIn. simpl_pfunc.
-        case_if => //. rewrite in_VVal => /eqP Hc.
-        rewrite -/pfunc. case_match => //.
-        * rewrite (nth_map "") => //.
-          rewrite nth_index. by simpl_pfunc.
-          by rewrite index_mem in H.
-        * move => /negP in H0. rewrite get_unioned_bot_setP in H0.
-          move => /negP /hasPn /(_ pfunc) in H0.
-          move => /eqP in H1. rewrite -pfunc_get_bot_setP in H1. rewrite H1 in H0.
-          rewrite mem_nth in H0. by move => /(_ is_true_true) in H0.
-          by case: (pf) => x_pf /= /eqP ->.
-      + rewrite /to_var_values_seq. rewrite (nth_map ""); last by autossr.
-        rewrite (nth_map ""); last by autossr.
-        rewrite t_update_neq => //.
-        apply /negP => /eqP Hv. subst.
-        rewrite index_uniq in Hi; try (by autossr).
-        by apply uniq_vars_in_program.
-  Qed.
-
-  Theorem transfer_inst_const_PFuncMapP :
-    forall p (pf: PFuncMap p) v c x_in x_out,
-      In _ (gamma pf) (x_in, x_out) ->
-      In _ (gamma (transfer_inst_const_PFuncMap pf v c)) (x_in, (v !-> c; x_out)).
-  Proof.
-    move => p pf v c x_in x_out HIn. move: (HIn) => HIn'.
-    apply /allP => i Hiota /=. move => /allP /(_ i Hiota) /= in HIn.
-    case Hindex: (size (vars_in_program p) <= index v (vars_in_program p)).
-    - rewrite /to_var_values_seq !(nth_map "") in HIn *; try (by autossr).
-      rewrite t_update_neq => [// | ].
-      apply /eqP => Hv. subst.
-      rewrite index_uniq in Hindex; simplssr => //. by rewrite leqNgt H in Hindex.
-      by apply uniq_vars_in_program.
-    - rewrite nth_set_nth /=.
-      case: (i =P index v (vars_in_program p)) => Hi. subst.
-      + rewrite /eval_pfunc. simpl_pfunc.
-        have ->: (to_var_values_seq p x_in \notin get_unioned_bot_set (sval pf)).
-          apply /negP. rewrite get_unioned_bot_set_pfuncmapP.
-          by move => /(_ x_out HIn').
-        rewrite (nth_map "") => //. rewrite t_update_eq_hyp. auto_pfunc.
-        rewrite nth_index => [ // | ].
-        by rewrite -index_mem.
-      + rewrite !(nth_map "") in HIn *; try by autossr.
-        rewrite t_update_neq => [ // | ].
-        apply /eqP => Hv. subst.
-        rewrite index_uniq in Hi => //. by autossr.
-        by apply uniq_vars_in_program.
-  Qed.
-
-  Theorem transfer_inst_const_PFuncMap_index :
-    forall p (pf: PFuncMap p) v c x_in x_out,
-      v \in vars_in_program p ->
-      In _ (gamma (transfer_inst_const_PFuncMap pf v c)) (x_in, x_out) ->
-      x_out v = c.
-  Proof.
-    move => p pf v c x_in x_out Hindex HIn.
-    move: (Hindex). rewrite -index_mem => Hindex_lt.
-    have Hiota: (index v (vars_in_program p)) \in iota 0 (size (vars_in_program p)) by simplssr.
-    move: HIn => /allP /(_ (index v (vars_in_program p)) Hiota) /=.
-    rewrite leqNgt Hindex_lt /= nth_set_nth /= eq_refl. rewrite /eval_pfunc. simpl_pfunc.
-    case_if => [ | //].
-    rewrite in_VVal => /eqP <-.
-    by rewrite to_var_values_seqP.
-  Qed.
-
-  Hint Resolve transfer_inst_const_PFuncMap_index : core.
-
-  Definition transfer_inst_PFuncMap {p: Program} (inst: Inst) (pf: PFuncMap p) :=
-    match inst with
-    | Const v c => transfer_inst_const_PFuncMap pf v c
-    | _ => pf
-    end.
-
-  Theorem transfer_inst_PFuncMapP :
-    forall p inst R R', inst_step inst R R' ->
-      forall (pf: PFuncMap p) R_begin, In _ (gamma pf) (R_begin, R) ->
-        In _ (gamma (transfer_inst_PFuncMap inst pf)) (R_begin, R').
-  Proof.
-    move => p inst R R' Hinst pf R_begin HIn.
-    case: inst Hinst => [ res c | res opc op1 op2 Hop1 Hop2 ] Hinst.
-    - inversion Hinst. subst.
-      eapply transfer_inst_const_PFuncMapP; eauto.
-    - admit.
-  Admitted.
-
-  Theorem transfer_inst_const_extract_dimension_apply_range_same :
-    forall p (pf: PFuncMap p) (x_in: RegisterMap) x_out res c (map: PMap (size (vars_in_program p)) _) i,
-      res \in (vars_in_program p) ->
-      i <> index res (vars_in_program p) ->
-      (to_var_values_seq p x_in, [:: x_out]) \in
-        (f_extract_dimension_map (f_apply_range_map map (pfuncmap_to_map pf)) i) ->
-        (to_var_values_seq p x_in, [:: x_out]) \in
-        (f_extract_dimension_map (f_apply_range_map map (pfuncmap_to_map (transfer_inst_const_PFuncMap pf res c))) i).
-    move => p pf x_in x_out res c map i Hres Hi_index.
-    move => /f_extract_dimension_mapP [x_out' [H_in_pf Hnth_xout']].
-    apply f_extract_dimension_mapP.
-    exists (set_nth 0%Z x_out' (index res (vars_in_program p)) c).
-    split; last first. rewrite nth_set_nth Hnth_xout' /=. autossr.
-    move: H_in_pf. rewrite_to_var_values_map_equality p x_out'.
-    move => /f_apply_range_mapP [x_mid /andP [Hin_map Hin_pf]].
-    apply f_apply_range_mapP. exists x_mid. apply /andP. split; auto.
-    rewrite -!pfuncmap_to_mapP in Hin_pf *.
-    move: Hin_map. rewrite_to_var_values_map_equality p x_mid. move => Hin_map.
-    move: (transfer_inst_const_PFuncMapP p pf res c (to_var_values_map p x_mid) (to_var_values_map p x_out')) => Htransfer.
-    erewrite gamma_seq_PFuncMap_equality in Hin_pf; first apply Htransfer in Hin_pf; simpl; auto; last by apply point_equality_refl.
-    rewrite /In /gamma /= /gamma_PFuncMap /= in Hin_pf.
-    erewrite gamma_seq_PFuncMap_equality; first apply Hin_pf; simpl; auto.
-    rewrite point_equality_sym. by apply to_var_values_seq_update.
-  Qed.
-
-  Theorem transfer_inst_extract_dimension_apply_range_res :
-    forall p (pf: PFuncMap p) (x_in: RegisterMap) x_out res c (map: PMap (size (vars_in_program p)) _),
-      res \in (vars_in_program p) ->
-      let i := index res (vars_in_program p) in
-      (to_var_values_seq p x_in, [:: x_out]) \in
-        (f_extract_dimension_map (f_apply_range_map map (pfuncmap_to_map pf)) i) ->
-        (to_var_values_seq p x_in, [:: c]) \in
-        (f_extract_dimension_map (f_apply_range_map map (pfuncmap_to_map (transfer_inst_const_PFuncMap pf res c))) i).
-  Proof.
-    move => p pf x_in x_out res c map Hres_in i.
-    move => /f_extract_dimension_mapP [x_out' [H_in_pf Hnth_xout']].
-    apply f_extract_dimension_mapP.
-    exists (set_nth 0%Z x_out' (index res (vars_in_program p)) c).
-    split; last by rewrite nth_set_nth /= eq_refl.
-    move: H_in_pf. rewrite_to_var_values_map_equality p x_out'.
-    move => /f_apply_range_mapP [x_mid /andP [Hin_map Hin_pf]].
-    apply f_apply_range_mapP. exists x_mid. apply /andP. split; auto.
-    rewrite -!pfuncmap_to_mapP in Hin_pf *.
-    move: Hin_map. rewrite_to_var_values_map_equality p x_mid. move => Hin_map.
-    move: (transfer_inst_const_PFuncMapP p pf res c (to_var_values_map p x_mid) (to_var_values_map p x_out')) => Htransfer.
-    erewrite gamma_seq_PFuncMap_equality in Hin_pf; first apply Htransfer in Hin_pf; simpl; auto; last by apply point_equality_refl.
-    rewrite /In /gamma /= /gamma_PFuncMap /= in Hin_pf.
-    erewrite gamma_seq_PFuncMap_equality; first apply Hin_pf; simpl; auto.
-    rewrite point_equality_sym. by apply to_var_values_seq_update.
-  Qed.
-
-
-  Theorem transfer_inst_compose_PFuncMapP :
-    forall p inst (pf comp_pf: PFuncMap p),
-      le (transfer_inst_PFuncMap inst (compose_relation comp_pf pf))
-         (compose_relation comp_pf (transfer_inst_PFuncMap inst pf)).
-  Proof.
-    move => p [ res c | res opc op1 op2 Hop1 Hop2 ] pf comp_pf [x_in x_out] HIn.
-    - case Hindex: (res \in (vars_in_program p)); last first.
-        rewrite -index_mem ltnNge in Hindex. move => /negb_false_iff in Hindex.
-        by rewrite /transfer_inst_PFuncMap !transfer_inst_PFuncMap_not_in_program in HIn *.
-      move: (HIn) => /transfer_inst_const_PFuncMap_exists [c' HIn'].
-      apply /allP => i Hiota. move: (HIn') => /allP /(_ i Hiota) /=.
-      rewrite !(nth_map 0); try (by rewrite size_iota; autossr).
-      rewrite map_to_pfuncP. move => [Heval | [x_out1 [x_out2 [Hx_ne [HIn1 HIn2]]]]].
-      + rewrite map_to_pfuncP. left.
-        rewrite nth_iota in Heval *; last by autossr. rewrite add0n in Heval *.
-        case: (i =P index res (vars_in_program p)) => Hi.
-        * subst. rewrite to_var_values_seqP => //.
-          rewrite (transfer_inst_const_PFuncMap_index p _ res c x_in x_out Hindex HIn).
-          by eapply transfer_inst_extract_dimension_apply_range_res; eauto.
-        * rewrite to_var_values_seq_update_neq in Heval; last by apply /eqP.
-          by apply transfer_inst_const_extract_dimension_apply_range_same.
-      + rewrite map_to_pfuncP.
-        case: (i =P index res (vars_in_program p)) => Hi.
-        * left. subst. rewrite to_var_values_seqP => //.
-          rewrite nth_iota in HIn1 HIn2 *; last by autossr. rewrite add0n in HIn1 HIn2 *.
-          rewrite (transfer_inst_const_PFuncMap_index p _ res c x_in x_out Hindex HIn).
-          by eapply transfer_inst_extract_dimension_apply_range_res; eauto.
-        * right. exists x_out1. exists x_out2. split; auto.
-          rewrite nth_iota in HIn1 HIn2 *; last by autossr.
-            by split; apply transfer_inst_const_extract_dimension_apply_range_same => //.
-    - admit.
-  Admitted.
 
 End PFuncMap.
